theories/sd_examples.v
@@ -704,14 +704,8 @@ Qed.
 
 Lemma wf_fields_wf  : map_Forall (λ _cname, wf_cdef_fields_wf) pdefs.
 Proof.
-  rewrite map_Forall_lookup => c0 d0.
-  rewrite lookup_insert_Some.
-  case => [[? <-]|[?]].
-  { by apply map_Forall_empty. }
-  rewrite lookup_singleton_Some.
-  case => [? <-].
-  apply map_Forall_singleton.
-  by repeat constructor.
+  apply: wf_cdef_fields_wf_context_correct.
+  exact (I <: True).
 Qed.
 
 Lemma wf_fields_mono : map_Forall (λ _cname, wf_field_mono) pdefs.
@@ -734,29 +728,8 @@ Qed.
 
 Lemma wf_methods_wf : map_Forall (λ _cname, wf_cdef_methods_wf) pdefs.
 Proof.
-  rewrite map_Forall_lookup => c0 d0.
-  rewrite lookup_insert_Some.
-  case => [[? <-]|[?]].
-  { rewrite /cdef_methods_bounded /ROBox /=.
-    apply map_Forall_singleton.
-    split.
-    { apply map_Forall_singleton.
-      by repeat constructor.
-    }
-    by repeat constructor.
-  }
-  rewrite lookup_singleton_Some => [[? <-]].
-  apply map_Forall_lookup => m mdef.
-  rewrite /Box /= lookup_insert_Some => [[[? <-] | ]].
-  - split.
-    { apply map_Forall_singleton.
-      by repeat constructor.
-    }
-    by repeat constructor.
-  - case => ?.
-    rewrite lookup_singleton_Some => [[? <-]].
-    split; first by apply map_Forall_empty.
-    by repeat constructor.
+  apply: wf_cdef_methods_wf_context_correct.
+  exact (I <: True).
 Qed.
 
 Lemma wf_methods_mono : map_Forall (λ _cname, wf_cdef_methods_mono) pdefs.
@@ -871,12 +844,8 @@ Qed.
 
 Lemma wf_constraints_wf : map_Forall (λ _cname, wf_cdef_constraints_wf) pdefs.
 Proof.
-  rewrite map_Forall_lookup => c0 d0.
-  rewrite lookup_insert_Some.
-  case => [[? <-]|[?]].
-  { by rewrite /wf_cdef_constraints_wf /ROBox /= Forall_nil. }
-  rewrite lookup_singleton_Some => [[? <-]].
-  { by rewrite /wf_cdef_constraints_wf /Box /= Forall_nil. }
+  apply: wf_cdef_constraints_wf_context_correct.
+  exact (I <: True).
 Qed.
 
 Lemma wf_constraints_bounded : map_Forall (λ _cname, wf_cdef_constraints_bounded) pdefs.
